HMAC: Finalize the pure specification in the new style

crypto_hst/hmac/Hash.Sha256.Pure.fst
@@ -1,39 +1,28 @@
 module Hash.Sha256.Pure
 
-module U8 = FStar.UInt8
-module S8 = Hacl.UInt8
-module U32 = FStar.UInt32
-module S32 = Hacl.UInt32
-module U64 = FStar.UInt64
-module S64 = Hacl.UInt64
-module SB = Hacl.SBuffer
+module I8 = FStar.UInt8
+module I32 = FStar.UInt32
+module I64 = FStar.UInt64
+module IB = FStar.Buffer
+
 
 
 (* Define base types *)
-let u8 = FStar.UInt8.t
-let s8 = Hacl.UInt8.t
-let u32 = FStar.UInt32.t
-let s32 = Hacl.UInt32.t
-let uint32s = Seq.seq s32
-let bytes = Seq.seq s8
+let i8 = FStar.UInt8.t
+let i32 = FStar.UInt32.t
+let buf32 = Seq.seq i32
+let bytes = Seq.seq i8
 
 
 (* Define algorithm parameters *)
-let hl = 32ul
-let bl = 64ul
-let hashsize = hl
-let blocksize = bl
+let hashsize = 32ul
+let blocksize = 64ul
 
 
-(* Define SHA2 functions *)
+(* Define SHA2 *)
 
-assume val init : unit -> Tot (state:uint32s)
+//assume val init : unit -> Tot (state:buf32)
+//assume val update : (state:buf32) -> (data:bytes) -> Tot (state :buf32)
+//assume val finish : (state:buf32) -> Tot (Prims.tuple2 (hash:bytes{Seq.length hash = I32.v hashsize}) (state:buf32))
 
-assume val update : (state:uint32s) -> (data:bytes) -> (len:s32{Seq.length data = S32.v len})
-  -> Tot (state :uint32s)
-
-assume val finish : (state:uint32s)
-  -> Tot (Prims.tuple2 (hash:bytes{Seq.length hash = U32.v hashsize}) (state:uint32s))
-
-assume val sha256 : (data:bytes) -> (len:s32{Seq.length data = S32.v len})
-  -> Tot (hash:bytes{Seq.length hash = U32.v hashsize})
+assume val sha256 : (data:bytes) -> Tot (hash:bytes{Seq.length hash = I32.v hashsize})
